mark-and-sweep/spec/GC.Spec.ChunkedMajorGC.Graph.fsti
@@ -55,6 +55,12 @@ val chunked_major_successors_preserved
   (x: obj_addr)
   : prop
 
+val chunked_major_live_subgraph_preserved
+  (mh_init: MH.major_heap)
+  (mh_final: MH.major_heap)
+  (live: obj_addr -> prop)
+  : prop
+
 val chunked_major_successors_preserved_elim
   (mh_init: MH.major_heap)
   (mh_final: MH.major_heap)
@@ -65,6 +71,48 @@ val chunked_major_successors_preserved_elim
         forall (y: obj_addr).
           chunked_major_edge mh_init x y <==>
           chunked_major_edge mh_final x y)
+
+val chunked_major_live_subgraph_preserved_intro
+  (mh_init: MH.major_heap)
+  (mh_final: MH.major_heap)
+  (live: obj_addr -> prop)
+  : Lemma
+      (requires
+        (forall (x: obj_addr).
+          live x ==>
+          chunked_major_vertex mh_init x /\
+          chunked_major_vertex mh_final x) /\
+        (forall (x: obj_addr).
+          live x ==>
+          forall (y: obj_addr).
+          (chunked_major_edge mh_init x y <==>
+           chunked_major_edge mh_final x y)))
+      (ensures chunked_major_live_subgraph_preserved mh_init mh_final live)
+
+val chunked_major_live_subgraph_vertices_elim
+  (mh_init: MH.major_heap)
+  (mh_final: MH.major_heap)
+  (live: obj_addr -> prop)
+  : Lemma
+      (requires chunked_major_live_subgraph_preserved mh_init mh_final live)
+      (ensures
+        forall (x: obj_addr).
+          live x ==>
+          chunked_major_vertex mh_init x /\
+          chunked_major_vertex mh_final x)
+
+val chunked_major_live_subgraph_edges_elim
+  (mh_init: MH.major_heap)
+  (mh_final: MH.major_heap)
+  (live: obj_addr -> prop)
+  : Lemma
+      (requires chunked_major_live_subgraph_preserved mh_init mh_final live)
+      (ensures
+        forall (x: obj_addr).
+          live x ==>
+          forall (y: obj_addr).
+          (chunked_major_edge mh_init x y <==>
+           chunked_major_edge mh_final x y))
 
 val chunked_major_vertex_single_chunk_compat
   (g: heap)
